%%%%%%%%%%%%%%%%%%%%%%%%%%%%%%%%%%%%%%%%%%%%%%%%%%%%%%%%%%%%%%%%%%%%%%
% writeLaTeX Example: A quick guide to LaTeX
%
% Source: Dave Richeson (divisbyzero.com), Dickinson College
% 
% A one-size-fits-all LaTeX cheat sheet. Kept to two pages, so it 
% can be printed (double-sided) on one piece of paper
% 
% Feel free to distribute this example, but please keep the referral
% to divisbyzero.com
% 
%%%%%%%%%%%%%%%%%%%%%%%%%%%%%%%%%%%%%%%%%%%%%%%%%%%%%%%%%%%%%%%%%%%%%%
% How to use writeLaTeX: 
%
% You edit the source code here on the left, and the preview on the
% right shows you the result within a few seconds.
%
% Bookmark this page and share the URL with your co-authors. They can
% edit at the same time!
%
% You can upload figures, bibliographies, custom classes and
% styles using the files menu.
%
% If you're new to LaTeX, the wikibook is a great place to start:
% http://en.wikibooks.org/wiki/LaTeX
%
%%%%%%%%%%%%%%%%%%%%%%%%%%%%%%%%%%%%%%%%%%%%%%%%%%%%%%%%%%%%%%%%%%%%%%

\documentclass[10pt,landscape]{article}
\usepackage{amssymb,amsmath,amsthm,amsfonts}
\usepackage{multicol,multirow, graphicx}
\usepackage{calc}
\usepackage{ifthen}
\usepackage[landscape]{geometry}
\usepackage[colorlinks=true,citecolor=blue,linkcolor=blue]{hyperref}
\usepackage{enumitem}
\usepackage{parskip, bm}


\ifthenelse{\lengthtest { \paperwidth = 11in}}
    { \geometry{top=.25in,left=.25in,right=.25in,bottom=.25in} }
	{\ifthenelse{ \lengthtest{ \paperwidth = 297mm}}
		{\geometry{top=1cm,left=1cm,right=1cm,bottom=1cm} }
		{\geometry{top=1cm,left=1cm,right=1cm,bottom=1cm} }
	}
\pagestyle{empty}
\makeatletter
\renewcommand{\section}{\@startsection{section}{1}{0mm}%
                                {-1ex}% plus -.5ex minus -.2ex}%
                                {0.5ex}% plus .2ex}%x
                                {\normalfont\large\bfseries}}
\renewcommand{\subsection}{\@startsection{subsection}{2}{0mm}%
                                {-1ex}% plus -.5ex minus -.2ex}%
                                {0.5ex}% plus .2ex}%
                                {\normalfont\normalsize\bfseries}}
\renewcommand{\subsubsection}{\@startsection{subsubsection}{3}{0mm}%
                                {-1ex}% plus -.5ex minus -.2ex}%
                                {1ex}% plus .2ex}%
                                {\normalfont\small\bfseries}}
\makeatother
\setcounter{secnumdepth}{0}
\setlength{\parskip}{3pt}
\setlength{\parindent}{-0.2in}
\setlength{\leftskip}{0.2in}


\setlist[itemize]{noitemsep, topsep=0pt, leftmargin= 0.5cm}
\setlist[enumerate]{noitemsep, topsep=0pt, leftmargin= 0.5cm}


\newcommand{\norm}[1]{\left\lVert#1\right\rVert}
\def\mystrut(#1,#2){\vrule height #1pt depth #2pt width 0pt}

\allowdisplaybreaks[4]
\let \ds \displaystyle
\makeatletter
\newcommand*{\rom}[1]{\expandafter\@slowromancap\romannumeral #1@}
\makeatother



% -----------------------------------------------------------------------

\begin{document}

\raggedright
\footnotesize

\begin{center}
     \Large{\textbf{CME 102 ACE -- Final Exam Reference Sheet}} \\
\end{center}
\begin{multicols}{3}
\setlength{\premulticols}{1pt}
\setlength{\postmulticols}{1pt}
\setlength{\multicolsep}{1pt}
\setlength{\columnsep}{2pt}
\section{First-Order ODE}
\subsection{Separation of Variables}
For any nonlinear first order ODE, manipulate to be in form $f(y)dy = g(x)dx$ then integrate.

\par Two special cases:
\begin{itemize}
\item ODE of form $y' = f(y/x)$, use $u = y/x$
\item ODE of form $y' = f(ay + bx + c)$, use $u = ay + bx + c$
\end{itemize}

\subsection{Linear Inhomogeneous}
ODEs of form $y' + p(x)y = r(x)$
\par Closed form solution:
\[ y(x) = e^{-\int p(x) dx} \left[ \int e^{\int p(x) dx} r(x)dx + C\right]\]
\textbf{Bernoulli Equation:} $y' + p(x) y = q(x)y^n$
\par Substitute $u = y^{1-n}$, solve $u' + (1-n)p(x) u = (1-n)q(x)$

\subsection{Eigenvalues/Eigenvectors}
For \textit{system} of ODEs of the form $\vec{x}' = \mathbf{A}\vec{x}$:
\begin{enumerate}
\item Assume solution $\vec{x}(t) = C\vec{v} e^{\lambda t}$ and plug in to find $\mathbf{A}\vec{v} = \lambda \vec{v}$

\item Solve for eigenvalues $\lambda$ of $\mathbf{A}$. For a 2x2 matrix $\mathbf{A} = \begin{bmatrix} a & b \\ c & d \end{bmatrix}$:
\[ \lambda = \frac{(a+d) \pm \sqrt{(a+d)^2 - 4(ad-bc)} }{2} \]

\item Solve for eigenvectors of $\mathbf{A}$. Special cases for 2x2 matrix:
\par \textbf{Case 1:} $c \neq 0$:
\[ \vec{v}_1 = \begin{bmatrix} \lambda_1 - d \\ c \end{bmatrix}, \; \vec{v}_2 = \begin{bmatrix} \lambda_2 -d \\ c \end{bmatrix} \]
\par \textbf{Case 2:} $b \neq 0$:
\[ \vec{v}_1 = \begin{bmatrix} b \\  \lambda_1 - a \end{bmatrix}, \; \vec{v}_2 = \begin{bmatrix} b \\ \lambda_2 - a \end{bmatrix} \]
\par \textbf{Case 3:} $b$ and $c$ are zero:
\[ \vec{v}_1 = \begin{bmatrix} 1 \\ 0 \end{bmatrix}, \; \vec{v}_2 = \begin{bmatrix} 0 \\ 1 \end{bmatrix} \]

\end{enumerate}

\section{Second-Order Nonlinear}
\subsection{``Missing y'' method}
\par Second order nonlinear ODE that does not contain $y$:
\[ F(y'', y', x) = 0\]
\begin{enumerate}
\item Make substitution $y' = u$ and $y'' = u'$ and rewrite ODE in terms of $u$ and $x$
\item Solve new ODE for $u(x)$
\item Find $y$ as $y = \int u(x) dx$
\end{enumerate}

\subsection{``Missing x'' method}
\par Second order nonlinear ODE that does not contain $x$:
\[ F(y'', y', y) = 0\]
\begin{enumerate}
\item Make substitution $y' = u$ and $y'' = u u'$ and rewrite ODE in terms of $u$ and $y$
\item Solve new ODE for $u(y)$
\item Substitute back $u = y'$ and solve for $y(x)$
\end{enumerate}

\section{Second-Order Linear Homogeneous}
Homogeneous solution has two \textbf{basis functions} $y_1$ and $y_2$. Write homogeneous solution as linear combination of these:
\[ y_h = C_1 y_1 + C_2 y_2 \]

\subsection{Variable Coefficients}
ODE has form:
\[ y'' + p(x) y' + q(x) y = 0\]
Solving using \textbf{reduction of order}. Given $y_1$, find $y_2$ as:
\[ y_2 = y_1 \int \frac{e^{-\int p dx}}{y_1^2} dx \]

\subsection{Constant Coefficients}
ODE has form:
\[ ay'' + by' + cy = 0 \]
with $a,\; b, \; c$ constant. Solve using \textbf{characteristic equation} $y = e^{\lambda x}$. Three cases:
\begin{description}
\item[Case 1] $b^2 - 4ac > 0$ (two distinct real roots):
\begin{gather*}
\lambda_1 = -\frac{b}{2a} + \frac{\sqrt{b^2 - 4ac}}{2a}, \quad \lambda_2 = -\frac{b}{2a} - \frac{\sqrt{b^2 - 4ac}}{2a} \\
y_h = C_1 e^{\lambda_1 x} + C_2 e^{\lambda_2 x}
\end{gather*}
\item[Case 2] $b^2 - 4ac = 0$ (double real root):
\[ \lambda = -\frac{b}{2a}, \quad y_h = (C_1 + C_2x) e^{\lambda x} \]
\item[Case 3] $b^2 - 4ac < 0$ (complex conjugate roots):
\begin{gather*}
\alpha = -\frac{b}{2a}, \quad \beta = \frac{\sqrt{4ac - b^2}}{2a}, \quad \lambda_{1,2} = \alpha \pm i\beta \\
y_h = e^{\alpha x}\left( C_1 \cos(\beta x) + C_2 \sin (\beta x)\right) 
\end{gather*}
\end{description}

\subsection{Euler-Cauchy equation}
ODE has form:
\[ ax^2y'' + bxy' + cy = 0 \]
with $a,\; b, \; c$ constant. Solve using \textbf{characteristic equation} $y = x^m$. Three cases:
\begin{description}
\item[Case 1] $(b-a)^2 - 4ac > 0$:
\begin{gather*}
m_{1,2} = -\frac{b-a}{2a} \pm \frac{\sqrt{(b-a)^2 - 4ac}}{2a} \\
y_h = C_1 x^{m_1} + C_2 x^{m_2}
\end{gather*}
\item[Case 2] $(b-a)^2 - 4ac = 0$:
\[ m = -\frac{b-a}{2a}, \quad y_h = (C_1 + C_2\ln|x|) x^m \]
\item[Case 3] $(b-a)^2 - 4ac < 0$:
\begin{gather*}
\alpha = -\frac{b-a}{2a}, \quad \beta = \frac{\sqrt{4ac - (b-a)^2}}{2a}, \quad m_{1,2} = \alpha \pm i\beta \\
y_h = x^\alpha \left( C_1 \cos(\beta \ln|x|) + C_2 \sin(\beta \ln|x|) \right) 
\end{gather*}
\end{description}


\section{Second-Order Linear Inhomogeneous}
\begin{itemize}
\item You \textbf{must} always solve for the homogeneous solution first
\item The final solution is $y = y_h + y_p$
\item Apply initial conditions \textbf{after} finding the particular solution
\end{itemize}

\subsection{Variation of Parameters}
\begin{itemize}
\item Must use for variable coefficient second order linear ODE
\item Integrals are hard, so only use if undetermined coefficients does not apply
\end{itemize}

\begin{enumerate}
\item Find homogeneous basis solutions $y_1$ and $y_2$
\item Calculate Wronskian:
\[ W = y_1 y_2' - y_2 y_1' \]
\item Put ODE into standard form:
\[ y'' + p(x)y' + q(x)y = r(x) \]
\item Calculate the particular solution:
\[ y_p = -y_1 \int \frac{y_2 r}{W} dx + y_2 \int \frac{y_1 r}{W} dx \]
\end{enumerate}


\subsection{Undetermined Coefficients}
\begin{itemize}
\item Only applicable to constant coefficient equations
\item If you need to solve for more than $\sim4$ constants, variation of parameters probably faster
\end{itemize}

\begin{enumerate}
\item Find homogeneous basis solutions $y_1$ and $y_2$
\item Put ODE into standard form:
\[ y'' + by' + cy = r(x) \]
\item Guess particular solution $y_p(x)$ based on table:
\begin{flalign*}
&\text{Form for $r(x)$:} & \text{Pick $y_p(x)$:} \\
& C \quad &A \\
& x^n & A_n x^n + A_{n-1} x^{n-1} + \cdots + A_1 x + A_0 \\
&e^{\gamma x} & Ae^{\gamma x} \\
& \cos(\omega x) \text{ or } \sin(\omega x) & A\cos(\omega x) + B\sin(\omega x) \\
\end{flalign*}
\begin{itemize}
\item Can have products of these functions (but only these functions) for $r(x)$ and the assumed solution
\item If any part of assumed solution also part of homogeneous basis, apply \textbf{modification rule} by multiplying assumed solution by $x$
\item Sometimes need to use trig identities to make $r(x)$ match something in the table
\end{itemize}
\item Take derivatives of assumed $y_p(x)$ and plug into ODE
\item Algebraically solve for the constants in assumed solution
\end{enumerate}

\section{Circuits}
Kirchoff's voltage law: $\sum_i V_i = 0$ i.e. sum of all voltage drops across elements is zero (conservation of energy)
\par To form circuit equations:
\begin{enumerate}
\item Apply Kirchoff's voltage law around loop (or loops)
\begin{itemize}
\item If there are multiple voltage loops i.e. you are forming a system of ODEs, make sure loops do not overlap
\end{itemize}
\item If there is a capacitor (and therefore $\int_0^t i(\tau)d\tau$ appears in the equation), take derivation through equation to form second order ODE
\item Solve second order linear ODE using Laplace transform or other method
\end{enumerate}

Voltage drops for elements:
\begin{itemize}
\item Inductor: $v = Li'$
\item Resistor: $v = Ri$ (Ohm's law)
\item Capactor: $v = \frac{Q}{C} = \frac{\int_0^t i(\tau)d\tau}{C}$ (charge over capacitance)
\end{itemize}

%\section{Spring-mass Systems}
%All equations start with force balance (Newton's second law):
%\[ \sum_i F_i = mx''\]
%Equation will look like:
%\[ mx''  + \beta x' + kx = 0\]
%\begin{itemize}
%\item $\beta$ is damping coefficient ($\beta = 0$ means undamped motion)
%\item $k$ is spring constant 
%\item $x(t)$ is the \textit{displacement} from the equilibrium position $x_0$
%\end{itemize}
%Rewrite ODE as: $x'' + 2 \mu + \omega^2 x = 0 $. 
%\par \textbf{Undamped motion:} $x(t) = A \sin (\omega t) + B \cos(\omega t)$
%\par \textbf{Damped motion:} when $\beta \neq 0$:
%\begin{description}
%\item[Over Damped:] $\mu > \omega$, 
%\[ x(t) = C_1 e^{(-\mu + \sqrt{\mu^2 - \omega^2})t} + C_2 e^{(-\mu - \sqrt{\mu^2 - \omega^2})t} \]
%\item[Critically Damped:] $\mu = \omega$, shortest decay time
%\[ x(t) = e^{-\mu t}(C_1 + C_2 t) \]
%\item[Underdamped:] $\mu < \omega$, 
%\[ x(t) = e^{-\mu t} \left[ C_1 \cos(\sqrt{\omega^2 - \mu^2} t) + C_2 \sin (\sqrt{\omega^2 - \mu^2}t) \right] \]
%\end{description}


\section{Numerical Methods for IVP's}

\subsection{Accuracy}
\begin{itemize}
\item Local error: error incurred over one step
\item Global error: total error over the domain, one order of $h$ less than local error, calculated as $\epsilon_{global} = N \times \epsilon_{local}$
\end{itemize}

\subsection{Stability}
\begin{itemize}
\item Derive amplification factor $\sigma(h)$ by starting with the model equation $y' = \lambda y$ and ``stepping-through'' the numerical method to derive relationship:
\[ y_{n+1} = \sigma(h) y_n\]
\item Stability condition is $|\sigma(h)| < 1$
\item To find stable $h$, solve $\sigma(h) < 1$ and $\sigma(h) > -1$
\end{itemize}

\subsection{Euler}
\textbf{Forward Euler:} explicit, $\mathcal{O}(h)$ global accuracy:
\[ y_{n+1} = y_n + h f(x_n, y_n) \]
\textbf{Backward Euler:} implicit, $\mathcal{O}(h)$ global accuracy:
\[ y_{n+1} = y_n + h f(x_{n+1}, y_{n+1}) \]

\subsection{Runge-Kutta Methods}
\textbf{Trapezoidal:} implicit, $\mathcal{O}(h^2)$ global accuracy, related to RK2, average of backward and forward Euler:
\[ y_{n+1} = y_n + \frac{h}{2} \left[ f(x_n, y_n) + f(x_{n+1}, y_{n+1})\right] \]
\textbf{Improved Euler/RK2:} explicit, $\mathcal{O}(h^2)$ global accuracy:
\[ y_{n+1} = y_n + \frac{h}{2} \left[ f(x_n, y_n) + f(x_{n+1}, y_n + h f(x_n,y_n))\right] \]
\textbf{RK4:} explicit, $\mathcal{O}(h^4)$ global accuracy, basis of \texttt{ode45()}:
\begin{gather*}
k_1 = f(t_n, y_n) \\
k_2 = f\left(t_n + \frac{h}{2}, y_n + \frac{h}{2} k_1\right) \\
k_3 = f\left(t_n + \frac{h}{2}, y_n + \frac{h}{2} k_2\right) \\
k_4 = f\left(t_n + h, y_n + hk_3\right) \\
y_{n+1} = y_n + h\left( \frac{1}{6} k_1 + \frac{1}{3} k_2 + \frac{1}{3} k_3 + \frac{1}{6} k_4 \right) 
\end{gather*}


\subsection{Higher-Order Systems of ODEs}
\begin{itemize}
\item ODEs (or systems of ODEs) that contain higher than first derivatives
\item Need to convert to first order to apply numerical methods
\end{itemize}
Create table:
\[ [\text{Old}]\quad |\quad [\text{New}]\quad | \quad [\text{Derivative}] \quad | \quad [\text{New ODE}] \]

\subsection{Multi-Step Methods}
\begin{itemize}
\item Uses information from multiple time steps to find next step. 
\item Methods are \textbf{not self-starting}
\end{itemize}

\par \textbf{Adams-Bashforth:} $y_{n+1} = y_n  + \frac{h}{2} [3f_n - f_{n-1}]$, second order accurate


%\par \textbf{Adams-Moulton:} ``predictor-corrector''. Second order: 
%\begin{gather*}
%\tilde{y}_{n+1} = y_n  + \frac{h}{2} [3f_n - f_{n-1}] \quad \text{predictor} \\
%y_{n+1} = y_n + \frac{h}{2} [ f(t_n,y_n) + f(t_{n+1}, \tilde{y}_{n+1})]
%\end{gather*}

\section{Numerical Methods for BVP's}
\subsection{Finite differences}
First derivatives
\begin{itemize}
\item Forward difference: $y'_i = \frac{y_{i+1} - y_i}{h}$, $\mathcal{O}(h)$ error
\item Backward difference: $y'_i = \frac{y_{i} - y_{i-1}}{h}$, $\mathcal{O}(h)$ error
\item Central difference: $y'_i = \frac{y_{i+1} - y_{i-1}}{2h}$, $\mathcal{O}(h^2)$ error
\end{itemize}
Second derivative: use second order central difference:
\[ y_i'' = \frac{y_{i+1} - 2y_i + y_{i-1}}{h^2}, \; \mathcal{O}(h^2) \text{ error} \]

\subsection{Boundary Conditions}
\begin{itemize}
\item Dirichlet: value given (e.g. $y(x_L) = C$)
\item Neuman: derivative given (e.g. $y'(x_L) = C$)
\item Robin: combination of value and derivative (e.g. $y'(x_L) + \alpha y(x_L) = C$)
\end{itemize}

\subsection{Setting Up Direct Method Equations}
\begin{enumerate}
\item Replace derivatives in ODE with finite difference approximations, and group coefficients of $y_{i-1}$, $y_i$, and $y_{i+1}$ to find \textit{recursive equation}

\item Treat boundary conditions
\begin{enumerate}
\item \textbf{Dirichlet (value given):} plug boundary value (at $y_1$ or $y_N$) into recursive equation at node next to boundary (either $i=2$ or $i=N-1$)
\item \textbf{Robin or Neuman (includes derivative):} plug finite difference approximation for $y'$ into the boundary condition, solve out for the ghost point, plug into recursive equation at the boundary node (either $i=1$ or $i=N$)
\end{enumerate}

\item Assemble system of equations in form $\mathbf{A} \vec{y} = \vec{f}$

\end{enumerate}

\subsection{Shooting Method}
Main idea: treat BVP like IVP
\begin{enumerate}
\item Guessing the initial condition we don't know at left boundary
\item Solve ODE using method for IVP
\item Update guess for initial condition based on error at right boundary
\item Iterate until error is zero
\end{enumerate}

\section{MATLAB}
\par \texttt{[t,y] = ode45(@(t,y) myODE(t,y), tspan, y0)}
\par If \texttt{myODE} has two arguments: \texttt{[t,y] = ode45(@myODE, tspan, y0)}
\par Anonymous function: \texttt{f = @(x) [expression]}

\section{Trigonometric Identities}
\par \textbf{Regular trigonometric identities:}
\begin{gather*}
\sin^2 x + \cos^2 x = 1, \; \tan^2 x + 1 = \sec^2 x, 1 + \cot^2 x = \csc^2 x \\
\sin (2x) = 2 \sin x \cos x, \; \tan(2x) = \frac{ 2 \tan x}{1 - \tan^2 x}\\
\cos (2x) = \cos^2 x - \sin^2 x = 2 \cos^2 x - 1 = 1 - 2 \sin^2 x
\end{gather*}

\par \textbf{Hyperbolic trigonometric functions:}
\begin{gather*}
\sinh x = \frac{ e^x - e^{-x}}{2}, \; \cosh x = \frac{ e^x + e^{-x}}{2}, \quad \tanh x  = \frac{e^x - e^{-x}}{e^x + e^{-x}} \\
\cosh^2 x - \sinh^2 x = 1, \; \tanh^2 x + \text{sech}^2 x = 1, \; \coth^2 x - \text{csch}^2 x = 1 \\
\sinh(2x) = 2 \sinh x \cosh x, \quad \cosh(2x) = 2 \cosh^2 x - 1\\
\tanh(2x) = \frac{ 2 \tanh x}{1 + \tanh^2 x}
\end{gather*}

\section{Useful Integrals/Derivatives}
\par \textbf{Trigonometric function derivatives:}
\begin{gather*}
\frac{d}{dx} \sin x = \cos x, \; \frac{d}{dx} \cot x = - \csc^2 x , \; \frac{d}{dx}\arcsin x = \frac{1}{\sqrt{1 - x^2}}\\
\frac{d}{dx}\cot x = - \sin x , \;\frac{d}{dx}\sec x = \sec x \tan x, \; \frac{d}{dx}\arccos x = \frac{ -1}{\sqrt{1 - x^2}}\\
\frac{d}{dx} \tan x = \sec^2 x , \; \frac{d}{dx} \csc x = - \csc x \cot x, \; \frac{d}{dx}\arctan x = \frac{1}{x^2 +1}
\end{gather*}

\par \textbf{Trigonometric and other integrals:}
\begin{gather*}
\int \tan x dx = - \log|\cos x| + C, \quad \int \cot x dx = \log | \sin x | + C \\
\int \csc x dx = - \log |\csc x + \cot x| + C \\
\int \sec x = \log |\sec x + \tan x| + C\\
\int \sin^2(x) dx = \frac{1}{2}x - \frac{1}{4} \sin(2x) + C \\
\int \cos^2(x)dx = \frac{1}{2} x + \frac{1}{4} \sin(2x) + C, \; \int \ln x dx = x \ln x - x + C \\
\int e^{ax} \sin (bx)dx = \frac{e^{ax}}{a^2 + b^2}(a \sin bx - b \cos bx) + C \\
\int e^{ax} \cos (bx)dx = \frac{e^{ax}}{a^2 + b^2}(a \cos bx + b \sin bx) + C 
\end{gather*}

\par \textbf{Inverse trigonometric function integrals:}
\begin{gather*}
\int \frac{dx}{x^2 + a^2} = \frac{1}{a} \arctan \frac{x}{a} + C, \; \int \frac{dx}{\sqrt{a^2 - x^2}} = \arcsin \frac{x}{a} + C 
\end{gather*}

\par \textbf{Hyperbolic trig function derivatives:}
\begin{gather*}
\frac{d}{dx} \sinh (x) = \cosh (x), \quad \frac{d}{dx}\cosh (x) = \sinh (x)\\
\frac{d}{dx}\tanh x = 1 - \tanh^2 (x), \quad \frac{d}{dx}\text{csch} (x) = - \text{coth}(x) \; \text{csch}(x) \\
\frac{d}{dx}\text{sech} (x) = - \tanh x \; \text{sech} (x), \quad
\frac{d}{dx}\coth x = 1 - \coth^2 (x)
\end{gather*}







%\section{Delimiters}
%\begin{tabular}{lll}
%\emph{description} & \emph{command} & \emph{output}\\
%parentheses &\verb!(x)! & (x)\\
%brackets &\verb![x]! & [x]\\
%curly braces& \verb!\{x\}! & \{x\}\\
%\end{tabular}


\end{multicols}

\end{document}
